Solutions

dot-simpler/dot-field-mut-stage-1/TransformExamples.v
@@ -24,6 +24,20 @@ subst_commut x y w z:
     (y <> w \/ x = z ) ->
     (subst_var x y) ∘ (subst_var w z) = (subst_var w (z \[x -> y])) ∘ (subst_var x y).
 
+Section AboutSubstCommut.
+  Context `(SC : SubstCommut A).
+  Lemma subst_commut' x y w z (X: A):
+    x <> w ->
+    (y <> w \/ x = z ) ->
+    (subst_var x y  (subst_var w z X)) = (subst_var w (z \[x -> y]) (subst_var x y X)).
+  Proof.
+    intros.
+    forwards Hsc: subst_commut; eauto.
+    unfold compose in Hsc.
+    eapply (fun_eq_1 X) in Hsc. auto.
+  Qed.
+End AboutSubstCommut.
+
 (* This property is easily proven for variables *)
 Instance AvarSubstCommut : SubstCommut AvarAbstractSyntax.
 Proof.
@@ -31,9 +45,69 @@ Proof.
   destruct H0; subst; contradiction. 
 Qed.
 
-(* 1.1 How to lift this property to types and terms? *)
+(* 1.1 How to lift this property to types and terms? - SOLVED *)
 
-(* 1.2 *)
+Section AboutTransformSyntax.
+  Context `{OA: Openable A} {FA: FreeVar A} {SA: SubstVar A}.
+  Context `{OB: Openable B} {FB: FreeVar B} {SB: SubstVar B}.
+  Context {ASB: AbstractSyntax OB FB SB} {ASA: AbstractSyntax OA FA SA}.
+  Context {C: Collect ASB ASA} {CC: CollectCompose C} {CR: CollectReflect C}
+          {FC: FvCollect C}.
+  Context {T: Transform ASB ASA} {TI: TransformId T} {TC: TransformCompose T}
+          {OT: OpenTransform T} {ST: SubstTransform T}.
+  Context {CT: CollectTransform C T}.
+
+  (** Every TransformSyntax leads to OpenCompose *)
+  Section SubstCommut.
+    Context {OTC: SubstCommut ASB}.
+    Instance TransformSubstCommut : SubstCommut ASA.
+    Proof.
+      hnf.
+      intros.
+
+      apply fun_ext_dep. intros a.
+      unfold compose.
+      rewrite ? (subst_depth 0).
+      rewrite subst_transform.
+      rewrite (subst_transform w z).
+      rewrite (subst_transform w (z \[ x -> y])).
+
+      rewrite ? fold_compose12. rewrite ? transform_compose.
+
+      eapply f_equal3; auto.
+      eapply fun_ext_nondep_2. intros.
+      rewrite <- fold_compose12.
+      rewrite <- fold_compose12.
+
+      rewrite <- (subst_depth).
+      rewrite <- (subst_depth).
+      rewrite <- (subst_depth).
+      rewrite <- (subst_depth).
+
+      eapply subst_commut'; eauto.
+    Qed.
+  End SubstCommut.
+End AboutTransformSyntax.
+Existing Instance TransformSubstCommut.
+
+(* These hints do not seem to help *)
+Hint Resolve TransformSubstCommut: core.
+Hint Resolve AvarSubstCommut: core.
+
+(* Test that the instance is found for types *)
+Lemma test_subst_commut_typ x y z w (t: typ):
+  x <> w ->
+  (y <> w \/ x = z ) ->
+  ((t /[ w -> z]) /[ x -> y]) = ((t /[ x -> y]) /[ w -> z \[ x -> y]]).
+Proof.
+  intros.
+  eapply subst_commut'; eauto.
+  (* For some reason, the instance is not found by eauto. *)
+  eapply TransformSubstCommut.
+Qed.
+
+
+(* 1.2 - WON'T PURSUE *)
 (* I have some other property where there is a precondition referring to the type or term, such as (closed X) *)
 (* For simplicity, i show it as a modification of the previous property *)
 Class ClosedSubstCommut `(AS : AbstractSyntax A) :=
@@ -48,7 +122,7 @@ subst_commut_closed x y w z (X: A):
 
 
 
-(* Question 2 *)
+(* Question 2 - SOLVED *)
 (* How to prove typ_bnd_close, which shows how closing distributes into typ_bnd? *)
 
 (* Similar lemma for opening typ_bnd proves easily *)
@@ -65,12 +139,87 @@ Proof.
   simpl. eauto.
 Qed.
 
-(* Here, the same approach does not work *)
+
+(* NEW CLASS for shifting the index in transform *)
+Class TransformShift `(AS : AbstractSyntax B) `(AS': AbstractSyntax A) (T: Transform AS AS'):=
+  transform_shift f X n m: transform f X (n + m) = transform (fun X' n' => f X' (n' + m)) X n.
+
+Lemma transform_shift_typ_dec (f : avar -> nat -> avar) :
+  (forall (X : typ) (n m : nat), transform f X (n + m) = transform (fun (X' : avar) (n' : nat) => f X' (n' + m)) X n) /\
+  (forall (X : dec) (n m : nat), transform f X (n + m) = transform (fun (X' : avar) (n' : nat) => f X' (n' + m)) X n).
+Proof.
+  apply typ_mutind; simpl; intros; try f_equal; auto.
+  - rewrite <- H. rewrite Nat.add_succ_l. auto.
+  - rewrite <- H0. rewrite Nat.add_succ_l. auto.
+Qed.
+
+Instance TypTransformShift : TransformShift TypTransform.
+Proof.
+  intro. eapply transform_shift_typ_dec.
+Qed.
+Instance DecTransformShift : TransformShift TypTransform.
+Proof.
+  intro. eapply transform_shift_typ_dec.
+Qed.
+
+Lemma transform_shift_terms (f : avar -> nat -> avar) :
+  (forall (X : trm) (n m : nat), transform f X (n + m) = transform (fun (X' : avar) (n' : nat) => f X' (n' + m)) X n) /\
+  (forall (X : lit) (n m : nat), transform f X (n + m) = transform (fun (X' : avar) (n' : nat) => f X' (n' + m)) X n) /\
+  (forall (X : def) (n m : nat), transform f X (n + m) = transform (fun (X' : avar) (n' : nat) => f X' (n' + m)) X n) /\
+  (forall (X : defs) (n m : nat), transform f X (n + m) = transform (fun (X' : avar) (n' : nat) => f X' (n' + m)) X n).
+Proof.
+  apply trm_mutind; simpl; intros; try f_equal; auto.
+  - rewrite <- H0. rewrite Nat.add_succ_l. auto.
+  - rewrite <- H0. rewrite Nat.add_succ_l. auto.
+  - rewrite <- transform_shift. auto.
+  - rewrite <- H. rewrite Nat.add_succ_l. auto.
+  - rewrite <- transform_shift. auto.
+  - rewrite <- H. rewrite Nat.add_succ_l. auto.
+  - rewrite <- transform_shift. auto.
+Qed.
+
+Instance TrmTransformShift : TransformShift TrmTransform.
+Proof.
+  intro. eapply transform_shift_terms.
+Qed.
+Instance LitTransformShift : TransformShift LitTransform.
+Proof.
+  intro. eapply transform_shift_terms.
+Qed.
+Instance DefTransformShift : TransformShift DefsTransform.
+Proof.
+  intro. eapply transform_shift_terms.
+Qed.
+Instance DefsTransformShift : TransformShift DefsTransform.
+Proof.
+  intro. eapply transform_shift_terms.
+Qed.
+
+
+(* Now, we can prove this lemma *)
 Lemma typ_bnd_close n x T1:
   close_rec n x (typ_bnd T1) = typ_bnd (close_rec (S n) x T1).
 Proof.
-  simpl. eauto.
-  (* even compute tactic does not help *)
-  compute. eauto.
-Qed.
+  sympl.
+  unfold TransformClosing; sympl.
+  unfold close_rec, transform, TypTransform.
 
+  eapply f_equal. (* Strips typ_bnd *)
+  (* Here we get the goal:
+   transform_typ (close_depth_rec n x) T1 1 = transform_typ (close_depth_rec (S n) x) T1 0 *)
+  replace 1 with (0 + 1). (* Puts the number into a form that transform_shift understands *)
+  rewrite rewrite_transform_typ. (* Folds transform_typ into transform *)
+  rewrite transform_shift.
+  eapply f_equal3; auto. (* Strips transform *)
+  eapply fun_ext_nondep_2.
+    intros. unfold close_depth_rec.
+    eapply f_equal3; auto. (* Strips close_rec *)
+    rewrite Nat.add_succ_l.
+    rewrite Nat.add_succ_r.
+    rewrite Nat.add_succ_r.
+    rewrite Nat.add_0_r.
+    auto.
+  (* 0 + 1 *)
+  rewrite Nat.add_0_l.
+  auto.
+Qed.
